@prefix : <http://w3id.org/ado#> .
@prefix ado: <http://w3id.org/ado/> .
@prefix owl: <http://www.w3.org/2002/07/owl#> .
@prefix pmd: <https://w3id.org/pmd/co/> .
@prefix rdf: <http://www.w3.org/1999/02/22-rdf-syntax-ns#> .
@prefix xml: <http://www.w3.org/XML/1998/namespace> .
@prefix xsd: <http://www.w3.org/2001/XMLSchema#> .
@prefix rdfs: <http://www.w3.org/2000/01/rdf-schema#> .
@prefix schema: <http://schema.org/> .
@prefix dcterms: <http://purl.org/dc/terms/> .
@base <http://w3id.org/ado> .

<http://w3id.org/ado> rdf:type owl:Ontology ;
                       dcterms:creator "Anastasia Dimou"@en ,
                                       "Ioannis Dasoulas"@en ;
                       dcterms:license "The Adhesives Ontology"@en ,
                                       "http://creativecommons.org/licenses/by/2.0/"^^xsd:anyURI ;
                       owl:versionInfo "1.0.0"@en .

#################################################################
#    Annotation properties
#################################################################

###  http://purl.org/dc/terms/creator
dcterms:creator rdf:type owl:AnnotationProperty .


###  http://purl.org/dc/terms/license
dcterms:license rdf:type owl:AnnotationProperty .


###  http://purl.org/dc/terms/title
dcterms:title rdf:type owl:AnnotationProperty .


#################################################################
#    Object Properties
#################################################################

###  http://schema.org/brand
schema:brand rdf:type owl:ObjectProperty .


###  http://w3id.org/ado/adhesionApplication
ado:adhesionApplication rdf:type owl:ObjectProperty ;
                        rdfs:domain ado:AdhesiveFamily ;
                        rdfs:range ado:AdhesionApplication ;
                        rdfs:comment "A relation between an adhesive family and a type of application it is commonly used in" .


###  http://w3id.org/ado/adhesionQuality
ado:adhesionQuality rdf:type owl:ObjectProperty ;
                    rdfs:domain ado:AdhesiveFamily ;
                    rdfs:range ado:AdhesionQuality ;
                    rdfs:comment "A relation between an adhesive type and the quality of adhesion it achieves with a material family." .


###  http://w3id.org/ado/adhesionQualityMaterialFamily
ado:adhesionQualityMaterialFamily rdf:type owl:ObjectProperty ;
                                  rdfs:domain ado:AdhesionQuality ;
                                  rdfs:range ado:MaterialFamily ;
                                  rdfs:comment "A relation between an adhesion quality estimation for an adhesive type and the material family the estimation corresponds to." .


###  http://w3id.org/ado/adhesiveFamily
ado:adhesiveFamily rdf:type owl:ObjectProperty ;
                   rdfs:domain ado:Adhesive ;
                   rdfs:range ado:AdhesiveFamily ;
                   rdfs:comment "A relation between an adhesive and the adhesive family it belongs to." .


###  http://w3id.org/ado/baseMaterial
ado:baseMaterial rdf:type owl:ObjectProperty ;
                 rdfs:domain ado:Substrate ;
                 rdfs:range pmd:PMD_0000000 ;
                 rdfs:comment "A relation between a substrate and the base material it consists of" .


###  http://w3id.org/ado/ceramicAdhesionQuality
ado:ceramicAdhesionQuality rdf:type owl:ObjectProperty ;
                           rdfs:subPropertyOf ado:adhesionQuality ;
                           rdfs:comment "A relation between an adhesive type and the quality of adhesion it achieves with ceramics." .


###  http://w3id.org/ado/compositeAdhesionQuality
ado:compositeAdhesionQuality rdf:type owl:ObjectProperty ;
                             rdfs:subPropertyOf ado:adhesionQuality ;
                             rdfs:comment "A relation between an adhesive type and the quality of adhesion it achieves with composites." .


###  http://w3id.org/ado/ferroMetalAdhesionQuality
ado:ferroMetalAdhesionQuality rdf:type owl:ObjectProperty ;
                              rdfs:subPropertyOf ado:adhesionQuality ;
                              rdfs:comment "A relation between an adhesive type and the quality of adhesion it achieves with ferrous metals." .


###  http://w3id.org/ado/glassAdhesionQuality
ado:glassAdhesionQuality rdf:type owl:ObjectProperty ;
                         rdfs:subPropertyOf ado:adhesionQuality ;
                         rdfs:comment "A relation between an adhesive type and the quality of adhesion it achieves with glass." .


###  http://w3id.org/ado/industry
ado:industry rdf:type owl:ObjectProperty ;
             rdfs:domain ado:AdhesionApplication ;
             rdfs:range ado:Industry ;
             rdfs:comment "A relation between an adhesion application and an industry it is commonly applied" .


###  http://w3id.org/ado/materialFamily
ado:materialFamily rdf:type owl:ObjectProperty ;
                   rdfs:domain ado:Substrate ;
                   rdfs:range ado:MaterialFamily ;
                   rdfs:comment "A relation between a substrate and the material family it is categorized as" .


###  http://w3id.org/ado/nonFerroMetalAdhesionQuality
ado:nonFerroMetalAdhesionQuality rdf:type owl:ObjectProperty ;
                                 rdfs:subPropertyOf ado:adhesionQuality ;
                                 rdfs:comment "A relation between an adhesive type and the quality of adhesion it achieves with non-ferrous metals." .


###  http://w3id.org/ado/resistantToSolvent
ado:resistantToSolvent rdf:type owl:ObjectProperty ;
                       rdfs:domain ado:Adhesive ;
                       rdfs:range ado:Solvent ;
                       rdfs:comment "A relation between an adhesive and a solvent it is resistant to" .


###  http://w3id.org/ado/rubberAdhesionQuality
ado:rubberAdhesionQuality rdf:type owl:ObjectProperty ;
                          rdfs:subPropertyOf ado:adhesionQuality ;
                          rdfs:comment "A relation between an adhesive type and the quality of adhesion it achieves with rubbers." .


###  http://w3id.org/ado/steelAdhesionQuality
ado:steelAdhesionQuality rdf:type owl:ObjectProperty ;
                         rdfs:subPropertyOf ado:adhesionQuality ;
                         rdfs:comment "A relation between an adhesive type and the quality of adhesion it achieves with steel." .


###  http://w3id.org/ado/thermoplasticAdhesionQuality
ado:thermoplasticAdhesionQuality rdf:type owl:ObjectProperty ;
                                 rdfs:subPropertyOf ado:adhesionQuality ;
                                 rdfs:comment "A relation between an adhesive type and the quality of adhesion it achieves with thermoplastic." .


###  http://w3id.org/ado/thermosetAdhesionQuality
ado:thermosetAdhesionQuality rdf:type owl:ObjectProperty ;
                             rdfs:subPropertyOf ado:adhesionQuality ;
                             rdfs:comment "A relation between an adhesive type and the quality of adhesion it achieves with thermoset." .


###  http://w3id.org/ado/woodAdhesionQuality
ado:woodAdhesionQuality rdf:type owl:ObjectProperty ;
                        rdfs:subPropertyOf ado:adhesionQuality ;
                        rdfs:comment "A relation between an adhesive type and the quality of adhesion it achieves with wood." .


#################################################################
#    Data properties
#################################################################

###  http://schema.org/color
schema:color rdf:type owl:DatatypeProperty .


###  http://schema.org/name
schema:name rdf:type owl:DatatypeProperty .


###  http://w3id.org/ado/adhesionQualityEstimation
ado:adhesionQualityEstimation rdf:type owl:DatatypeProperty ;
                              rdfs:domain ado:AdhesionQuality ;
                              rdfs:range xsd:string ;
                              rdfs:comment "A relation between an adhesion quality estimation entity and the relative value of the estimation" .


###  http://w3id.org/ado/adhesiveCost
ado:adhesiveCost rdf:type owl:DatatypeProperty ;
                 rdfs:domain ado:Adhesive ;
                 rdfs:range xsd:float ;
                 rdfs:comment "A relation between an adhesive and the estimation of its cost (in Euros) per mililiter (ml) based on amount paid for small scale tubes." .


###  http://w3id.org/ado/adhesiveMaxElongation
ado:adhesiveMaxElongation rdf:type owl:DatatypeProperty ;
                          rdfs:domain ado:Adhesive ,
                                      ado:AdhesiveFamily ;
                          rdfs:range xsd:float ;
                          rdfs:comment "A relation between an adhesive and its max elongation percentage" .


###  http://w3id.org/ado/chemicalDetachability
ado:chemicalDetachability rdf:type owl:DatatypeProperty ;
                          rdfs:domain ado:AdhesiveFamily ;
                          rdfs:range xsd:string ;
                          rdfs:comment "A relation between an adhesive family and its relative ability to be detached chemically" .


###  http://w3id.org/ado/chemicalResistance
ado:chemicalResistance rdf:type owl:DatatypeProperty ;
                       rdfs:subPropertyOf ado:environmentalResistance ;
                       rdfs:comment "A relation between an adhesive type or substrate and its relative ability to withstand chemicals" .


###  http://w3id.org/ado/complexModulus
ado:complexModulus rdf:type owl:DatatypeProperty ;
                   rdfs:domain ado:Adhesive ;
                   rdfs:range xsd:float ;
                   rdfs:comment "A relation between an adhesive and its resistance to deformation of the sample (in MPa)" .


###  http://w3id.org/ado/creepResistance
ado:creepResistance rdf:type owl:DatatypeProperty ;
                    rdfs:subPropertyOf ado:environmentalResistance ;
                    rdfs:comment "A relation between an adhesive type or substrate and its relative ability to withstand creep" .


###  http://w3id.org/ado/curingTimeEstimation
ado:curingTimeEstimation rdf:type owl:DatatypeProperty ;
                         rdfs:domain ado:AdhesiveFamily ;
                         rdfs:range xsd:string ;
                         rdfs:comment "A relation between an adhesive family and an estimation of time it requires to cure/harden" .


###  http://w3id.org/ado/eModulus
ado:eModulus rdf:type owl:DatatypeProperty ;
             rdfs:domain ado:Adhesive ;
             rdfs:range xsd:float ;
             rdfs:comment "A relation between an adhesive and its material's elasticity (in MPa)" .


###  http://w3id.org/ado/environmentalResistance
ado:environmentalResistance rdf:type owl:DatatypeProperty ;
                            rdfs:domain ado:AdhesiveFamily ,
                                        ado:Substrate ;
                            rdfs:range xsd:string ;
                            rdfs:comment "A relation between an adhesive type or a substrate and its relative ability to withstand environmental conditions" .


###  http://w3id.org/ado/fatigueStrengthLowerBound
ado:fatigueStrengthLowerBound rdf:type owl:DatatypeProperty ;
                              rdfs:domain ado:Substrate ;
                              rdfs:range xsd:float ;
                              rdfs:comment "A relation between a substrate and the lower bound of the highest stress that it can withstand for 10^7 cycles without breaking (in MPa)" .


###  http://w3id.org/ado/fatigueStrengthUpperBound
ado:fatigueStrengthUpperBound rdf:type owl:DatatypeProperty ;
                              rdfs:domain ado:Substrate ;
                              rdfs:range xsd:float ;
                              rdfs:comment "A relation between a substrate and the upper bound of the highest stress that it can withstand for 10^7 cycles without breaking (in MPa)" .


###  http://w3id.org/ado/freshWaterResistance
ado:freshWaterResistance rdf:type owl:DatatypeProperty ;
                         rdfs:subPropertyOf ado:environmentalResistance ;
                         rdfs:comment "A relation between an adhesive type or substrate and its relative ability to withstand fresh water" .


###  http://w3id.org/ado/humidityResistance
ado:humidityResistance rdf:type owl:DatatypeProperty ;
                       rdfs:subPropertyOf ado:environmentalResistance ;
                       rdfs:comment "A relation between an adhesive type or substrate and its relative ability to withstand humidity" .


###  http://w3id.org/ado/idealApplicationThickness
ado:idealApplicationThickness rdf:type owl:DatatypeProperty ;
                              rdfs:domain ado:Adhesive ;
                              rdfs:range xsd:float ;
                              rdfs:comment "A relation between an adhesive and the ideal thickness (in mm) it should be applied" .


###  http://w3id.org/ado/isMagnetic
ado:isMagnetic rdf:type owl:DatatypeProperty ;
               rdfs:domain ado:Substrate ;
               rdfs:range xsd:boolean ;
               rdfs:comment "A relation between a substrate and a value defining whether it is magnetic or not" .


###  http://w3id.org/ado/maxApplicationRelativeHumidity
ado:maxApplicationRelativeHumidity rdf:type owl:DatatypeProperty ;
                                   rdfs:domain ado:AdhesiveFamily ;
                                   rdfs:range xsd:float ;
                                   rdfs:comment "A relation between an adhesive type and its maximum relative humidity percentage" .


###  http://w3id.org/ado/maxApplicationTemperature
ado:maxApplicationTemperature rdf:type owl:DatatypeProperty ;
                              rdfs:domain ado:Adhesive ,
                                          ado:AdhesiveFamily ;
                              rdfs:range xsd:float ;
                              rdfs:comment "A relation between an adhesive  or a type of adhesives and the maximum temperature (in °C) it should be applied" .


###  http://w3id.org/ado/maxApplicationThickness
ado:maxApplicationThickness rdf:type owl:DatatypeProperty ;
                            rdfs:domain ado:Adhesive ;
                            rdfs:range xsd:float ;
                            rdfs:comment "A relation between an adhesive and the maximum thickness (in mm) it should be applied" .


###  http://w3id.org/ado/maxCuringTemperature
ado:maxCuringTemperature rdf:type owl:DatatypeProperty ;
                         rdfs:domain ado:AdhesiveFamily ;
                         rdfs:range xsd:float ;
                         rdfs:comment "A relation between an adhesive type and the maximum temperature it can be cured (in °C)" .


###  http://w3id.org/ado/maxDetachmentTemperature
ado:maxDetachmentTemperature rdf:type owl:DatatypeProperty ;
                             rdfs:domain ado:AdhesiveFamily ;
                             rdfs:range xsd:float ;
                             rdfs:comment "A relation between an adhesive family and the maximum temperature that can cause separation of the bonded parts (in °C)" .


###  http://w3id.org/ado/maxDissipationFactor
ado:maxDissipationFactor rdf:type owl:DatatypeProperty ;
                         rdfs:domain ado:Substrate ;
                         rdfs:range xsd:float ;
                         rdfs:comment "A relation between a substrate and an estimation of its maximum signal attenuation as the signal propagates down the transmission line (using dielectric loss tangent)" .


###  http://w3id.org/ado/maxElectricalConductivity
ado:maxElectricalConductivity rdf:type owl:DatatypeProperty ;
                              rdfs:domain ado:Substrate ;
                              rdfs:range xsd:float ;
                              rdfs:comment "A relation between a substrate and an estimation of its maximum reciprocal of electrical resistivity (in %IACS)" .


###  http://w3id.org/ado/maxGapFillingCapability
ado:maxGapFillingCapability rdf:type owl:DatatypeProperty ;
                            rdfs:domain ado:AdhesiveFamily ;
                            rdfs:range xsd:float ;
                            rdfs:comment "A relation between an adhesive family and its maximum estimated gap filling capability (in mm)" .


###  http://w3id.org/ado/maxGlassTemperature
ado:maxGlassTemperature rdf:type owl:DatatypeProperty ;
                        rdfs:domain ado:Substrate ;
                        rdfs:range xsd:float ;
                        rdfs:comment "A relation between a substrate and the maximum estimated temperature at which the glass transition can occur (in °C)" .


###  http://w3id.org/ado/maxGravityHardener
ado:maxGravityHardener rdf:type owl:DatatypeProperty ;
                       rdfs:domain ado:Adhesive ;
                       rdfs:range xsd:float ;
                       rdfs:comment "A relation between an adhesive and the maximum specific gravity or density of the hardener in g/cm³" .


###  http://w3id.org/ado/maxGravityResin
ado:maxGravityResin rdf:type owl:DatatypeProperty ;
                    rdfs:domain ado:Adhesive ;
                    rdfs:range xsd:float ;
                    rdfs:comment "A relation between an adhesive and the maximum specific gravity or density of the resin in g/cm³" .


###  http://w3id.org/ado/maxMeltingTemperature
ado:maxMeltingTemperature rdf:type owl:DatatypeProperty ;
                          rdfs:domain ado:Substrate ;
                          rdfs:range xsd:float ;
                          rdfs:comment "A relation between a substrate ant the maximum estimated temperature at which it changes state from solid to liquid (in °C)" .


###  http://w3id.org/ado/maxMixedViscosity
ado:maxMixedViscosity rdf:type owl:DatatypeProperty ;
                      rdfs:domain ado:Adhesive ;
                      rdfs:range xsd:float ;
                      rdfs:comment "A relation between an adhesive and its maximum viscosity of the hardener in mPa.s" .


###  http://w3id.org/ado/maxOpenTime
ado:maxOpenTime rdf:type owl:DatatypeProperty ;
                rdfs:domain ado:Adhesive ;
                rdfs:range xsd:float ;
                rdfs:comment "A relation between an adhesive and amount of time (in minutes) after its application to the substrate during which it retains its ability to adhere to and bond" .


###  http://w3id.org/ado/maxOperationalTemperature
ado:maxOperationalTemperature rdf:type owl:DatatypeProperty ;
                              rdfs:domain ado:AdhesiveFamily ;
                              rdfs:range xsd:float .


###  http://w3id.org/ado/maxPolymerTransitionTemperature
ado:maxPolymerTransitionTemperature rdf:type owl:DatatypeProperty ;
                                    rdfs:domain ado:Adhesive ;
                                    rdfs:range xsd:float ;
                                    rdfs:comment "Maximum estimated temperature at which amorphous polymers undergo a transition from glassy to rubbery state (in °C)" .


###  http://w3id.org/ado/maxPotLife
ado:maxPotLife rdf:type owl:DatatypeProperty ;
               rdfs:domain ado:Adhesive ;
               rdfs:range xsd:float ;
               rdfs:comment "A relation between an adhesive and the maximum period of time (in minutes) during which it maintains its workable properties after it's been mixed." .


###  http://w3id.org/ado/maxResistanceTemperature
ado:maxResistanceTemperature rdf:type owl:DatatypeProperty ;
                             rdfs:domain ado:Adhesive ;
                             rdfs:range xsd:float ;
                             rdfs:comment "A relation between an adhesive and the maximum temperature it can withstand (in °C)" .


###  http://w3id.org/ado/maxServiceTemperature
ado:maxServiceTemperature rdf:type owl:DatatypeProperty ;
                          rdfs:domain ado:Substrate ;
                          rdfs:range xsd:float ;
                          rdfs:comment "A relation between a substrate and the maximum estimated temperature at which it can be used in a load-bearing component without oxidation (in °C)" .


###  http://w3id.org/ado/maxShearStrength
ado:maxShearStrength rdf:type owl:DatatypeProperty ;
                     rdfs:domain ado:AdhesiveFamily ;
                     rdfs:range xsd:float ;
                     rdfs:comment "A relation between an adhesive type and its maximum estimated shear strength (in N/mm^2)" .


###  http://w3id.org/ado/maxSpecificHeatCapacity
ado:maxSpecificHeatCapacity rdf:type owl:DatatypeProperty ;
                            rdfs:domain ado:Substrate ;
                            rdfs:range xsd:float ;
                            rdfs:comment "A relation between a substrate and the maximum estimated amount of heat that must be added to one unit of its mass to cause an increase of one unit of temperature (in J/kg°C)" .


###  http://w3id.org/ado/maxStorageTemperature
ado:maxStorageTemperature rdf:type owl:DatatypeProperty ;
                          rdfs:domain ado:Adhesive ;
                          rdfs:range xsd:float ;
                          rdfs:comment "A relation between an adhesive and its maximum recommended storage temperature in °C" .


###  http://w3id.org/ado/maxSubstrateCost
ado:maxSubstrateCost rdf:type owl:DatatypeProperty ;
                     rdfs:domain ado:Substrate ;
                     rdfs:range xsd:float ;
                     rdfs:comment "A relation between a substrate and the maximum estimated cost to acquire a kilo of it in euros." .


###  http://w3id.org/ado/maxThermalConductivity
ado:maxThermalConductivity rdf:type owl:DatatypeProperty ;
                           rdfs:subPropertyOf ado:thermalConductivity ;
                           rdfs:comment "A relation between an adhesive or a substrate and a minimum estimation of its ability to conduct heat (in W/m.°C)" .


###  http://w3id.org/ado/maxThermalExpansionCoefficient
ado:maxThermalExpansionCoefficient rdf:type owl:DatatypeProperty ;
                                   rdfs:domain ado:Substrate ;
                                   rdfs:range xsd:float ;
                                   rdfs:comment "A relation between a substrate and an estimation of the maximum tendency of its matter to increase in length area, or volume in response to an increase in temperature (in μstrain/°C)" .


###  http://w3id.org/ado/maxToughness
ado:maxToughness rdf:type owl:DatatypeProperty ;
                 rdfs:domain ado:Substrate ;
                 rdfs:range xsd:float ;
                 rdfs:comment "A relation between a substrate and the maximum estimation of its ability to absorb energy and plastically deform without fracturing (in kJ/m^2)" .


###  http://w3id.org/ado/maxViscosityHardener
ado:maxViscosityHardener rdf:type owl:DatatypeProperty ;
                         rdfs:domain ado:Adhesive ;
                         rdfs:range xsd:float ;
                         rdfs:comment "A relation between an adhesive and its maximum viscosity of the hardener in mPa.s" .


###  http://w3id.org/ado/maxViscosityResin
ado:maxViscosityResin rdf:type owl:DatatypeProperty ;
                      rdfs:domain ado:Adhesive ;
                      rdfs:range xsd:float ;
                      rdfs:comment "A relation between an adhesive and its maximum viscosity of the resin in mPa.s" .


###  http://w3id.org/ado/maxWaterAbsorption
ado:maxWaterAbsorption rdf:type owl:DatatypeProperty ;
                       rdfs:domain ado:Substrate ;
                       rdfs:range xsd:float ;
                       rdfs:comment "A relation between a substrate and a maximum estimation of its ability to absorb water when immersed in it measured in percentage of water it absorbs in 24 hours" .


###  http://w3id.org/ado/maxWaterVaporTransmission
ado:maxWaterVaporTransmission rdf:type owl:DatatypeProperty ;
                              rdfs:domain ado:Substrate ;
                              rdfs:range xsd:float ;
                              rdfs:comment "A relation between a substrate and a maximum estimation of the passage of water vapor through it (in g*mm/m^2*day)" .


###  http://w3id.org/ado/mechanicalDetachability
ado:mechanicalDetachability rdf:type owl:DatatypeProperty ;
                            rdfs:domain ado:AdhesiveFamily ;
                            rdfs:range xsd:string ;
                            rdfs:comment "A relation between an adhesive family and its relative ability to be detached mechanically" .


###  http://w3id.org/ado/minApplicationRelativeHumidity
ado:minApplicationRelativeHumidity rdf:type owl:DatatypeProperty ;
                                   rdfs:domain ado:AdhesiveFamily ;
                                   rdfs:range xsd:float ;
                                   rdfs:comment "A relation between an adhesive type and its minimum relative humidity percentage" .


###  http://w3id.org/ado/minApplicationTemperature
ado:minApplicationTemperature rdf:type owl:DatatypeProperty ;
                              rdfs:domain ado:Adhesive ,
                                          ado:AdhesiveFamily ;
                              rdfs:range xsd:float ;
                              rdfs:comment "A relation between an adhesive  or a type of adhesives and the minimum temperature (in °C) it should be applied" .


###  http://w3id.org/ado/minApplicationThickness
ado:minApplicationThickness rdf:type owl:DatatypeProperty ;
                            rdfs:domain ado:Adhesive ;
                            rdfs:range xsd:float ;
                            rdfs:comment "A relation between an adhesive and the minimum thickness (in mm) it should be applied." .


###  http://w3id.org/ado/minCuringTemperature
ado:minCuringTemperature rdf:type owl:DatatypeProperty ;
                         rdfs:domain ado:AdhesiveFamily ;
                         rdfs:range xsd:float ;
                         rdfs:comment "A relation between an adhesive type and the minimum temperature it can be cured (in °C)" .


###  http://w3id.org/ado/minDetachmentTemperature
ado:minDetachmentTemperature rdf:type owl:DatatypeProperty ;
                             rdfs:domain ado:AdhesiveFamily ;
                             rdfs:range xsd:float ;
                             rdfs:comment "A relation between an adhesive family and the minimum temperature that can cause separation of the bonded parts (in °C)" .


###  http://w3id.org/ado/minDissipationFactor
ado:minDissipationFactor rdf:type owl:DatatypeProperty ;
                         rdfs:domain ado:Substrate ;
                         rdfs:range xsd:float ;
                         rdfs:comment "A relation between a substrate and an estimation of its minimum signal attenuation as the signal propagates down the transmission line (using dielectric loss tangent)" .


###  http://w3id.org/ado/minElectricalConductivity
ado:minElectricalConductivity rdf:type owl:DatatypeProperty ;
                              rdfs:domain ado:Substrate ;
                              rdfs:range xsd:float ;
                              rdfs:comment "A relation between a substrate and an estimation of its minimum reciprocal of electrical resistivity (in %IACS)" .


###  http://w3id.org/ado/minGapFillingCapability
ado:minGapFillingCapability rdf:type owl:DatatypeProperty ;
                            rdfs:domain ado:AdhesiveFamily ;
                            rdfs:range xsd:float ;
                            rdfs:comment "A relation between an adhesive family and its minimum estimated gap filling capability (in mm)" .


###  http://w3id.org/ado/minGlassTemperature
ado:minGlassTemperature rdf:type owl:DatatypeProperty ;
                        rdfs:domain ado:Substrate ;
                        rdfs:range xsd:float ;
                        rdfs:comment "A relation between a substrate and the minimum estimated temperature at which the glass transition can occur (in °C)" .


###  http://w3id.org/ado/minGravityHardener
ado:minGravityHardener rdf:type owl:DatatypeProperty ;
                       rdfs:domain ado:Adhesive ;
                       rdfs:range xsd:float ;
                       rdfs:comment "A relation between an adhesive and the minimum specific gravity or density of the hardener in g/cm³" .


###  http://w3id.org/ado/minGravityResin
ado:minGravityResin rdf:type owl:DatatypeProperty ;
                    rdfs:domain ado:Adhesive ;
                    rdfs:range xsd:float ;
                    rdfs:comment "A relation between an adhesive and the minimum specific gravity or density of the resin in g/cm³" .


###  http://w3id.org/ado/minMeltingTemperature
ado:minMeltingTemperature rdf:type owl:DatatypeProperty ;
                          rdfs:domain ado:Substrate ;
                          rdfs:range xsd:float ;
                          rdfs:comment "A relation between a substrate ant the minimum estimated temperature at which it changes state from solid to liquid (in °C)" .


###  http://w3id.org/ado/minMixedViscosity
ado:minMixedViscosity rdf:type owl:DatatypeProperty ;
                      rdfs:domain ado:Adhesive ;
                      rdfs:range xsd:float ;
                      rdfs:comment "A relation between an adhesive and its minimum viscosity of the hardener in mPa.s" .


###  http://w3id.org/ado/minOperationalTemperature
ado:minOperationalTemperature rdf:type owl:DatatypeProperty ;
                              rdfs:domain ado:AdhesiveFamily ;
                              rdfs:range xsd:float .


###  http://w3id.org/ado/minPolymerTransitionTemperature
ado:minPolymerTransitionTemperature rdf:type owl:DatatypeProperty ;
                                    rdfs:domain ado:Adhesive ;
                                    rdfs:range xsd:float ;
                                    rdfs:comment "Minimum estimated temperature at which amorphous polymers undergo a transition from glassy to rubbery state (in °C)" .


###  http://w3id.org/ado/minPotLife
ado:minPotLife rdf:type owl:DatatypeProperty ;
               rdfs:domain ado:Adhesive ;
               rdfs:range xsd:float ;
               rdfs:comment "A relation between an adhesive and the minimum estimate of the period of time (in minutes) during which it maintains its workable properties after it's been mixed." .


###  http://w3id.org/ado/minResistanceTemperature
ado:minResistanceTemperature rdf:type owl:DatatypeProperty ;
                             rdfs:domain ado:Adhesive ;
                             rdfs:range xsd:float ;
                             rdfs:comment "A relation between an adhesive and the minimum temperature it can withstand (in °C)" .


###  http://w3id.org/ado/minServiceTemperature
ado:minServiceTemperature rdf:type owl:DatatypeProperty ;
                          rdfs:domain ado:Substrate ;
                          rdfs:range xsd:float ;
                          rdfs:comment "A relation between a substrate and the minimum estimated temperature at which it can be used in a load-bearing component without oxidation (in °C)" .


###  http://w3id.org/ado/minShearStrength
ado:minShearStrength rdf:type owl:DatatypeProperty ;
                     rdfs:domain ado:AdhesiveFamily ;
                     rdfs:range xsd:float ;
                     rdfs:comment "A relation between an adhesive type and its minimum estimated shear strength (N/mm^2)" .


###  http://w3id.org/ado/minSpecificHeatCapacity
ado:minSpecificHeatCapacity rdf:type owl:DatatypeProperty ;
                            rdfs:domain ado:Substrate ;
                            rdfs:range xsd:float ;
                            rdfs:comment "A relation between a substrate and the minimum estimated amount of heat that must be added to one unit of its mass to cause an increase of one unit of temperature (in J/kg°C)" .


###  http://w3id.org/ado/minStorageTemperature
ado:minStorageTemperature rdf:type owl:DatatypeProperty ;
                          rdfs:domain ado:Adhesive ;
                          rdfs:range xsd:float ;
                          rdfs:comment "A relation between an adhesive and its minimum recommended storage temperature in °C" .


###  http://w3id.org/ado/minSubstrateCost
ado:minSubstrateCost rdf:type owl:DatatypeProperty ;
                     rdfs:domain ado:Substrate ;
                     rdfs:range xsd:float ;
                     rdfs:comment "A relation between a substrate and the minimum estimated cost to acquire a kilo of it in euros" .


###  http://w3id.org/ado/minThermalConductivity
ado:minThermalConductivity rdf:type owl:DatatypeProperty ;
                           rdfs:subPropertyOf ado:thermalConductivity ;
                           rdfs:comment "A relation between an adhesive or a substrate and a maximum estimation of its ability to conduct heat (in W/m.°C)" .


###  http://w3id.org/ado/minThermalExpansionCoefficient
ado:minThermalExpansionCoefficient rdf:type owl:DatatypeProperty ;
                                   rdfs:domain ado:Substrate ;
                                   rdfs:range xsd:float ;
                                   rdfs:comment "A relation between a substrate and an estimation of the minimum tendency of its matter to increase in length area, or volume in response to an increase in temperature (in μstrain/°C)" .


###  http://w3id.org/ado/minToughness
ado:minToughness rdf:type owl:DatatypeProperty ;
                 rdfs:domain ado:Substrate ;
                 rdfs:range xsd:float ;
                 rdfs:comment "A relation between a substrate and the minimum estimation of its ability to absorb energy and plastically deform without fracturing (in kJ/m^2)" .


###  http://w3id.org/ado/minViscosityHardener
ado:minViscosityHardener rdf:type owl:DatatypeProperty ;
                         rdfs:domain ado:Adhesive ;
                         rdfs:range xsd:float ;
                         rdfs:comment "A relation between an adhesive and its minimum viscosity of the hardener in mPa.s" .


###  http://w3id.org/ado/minViscosityResin
ado:minViscosityResin rdf:type owl:DatatypeProperty ;
                      rdfs:domain ado:Adhesive ;
                      rdfs:range xsd:float ;
                      rdfs:comment "A relation between an adhesive and its minimum viscosity of the resin in mPa.s" .


###  http://w3id.org/ado/minWaterAbsorption
ado:minWaterAbsorption rdf:type owl:DatatypeProperty ;
                       rdfs:domain ado:Substrate ;
                       rdfs:range xsd:float ;
                       rdfs:comment "A relation between a substrate and a minimum estimation of its ability to absorb water when immersed in it measured in percentage of water it absorbs in 24 hours" .


###  http://w3id.org/ado/minWaterVaporTransmission
ado:minWaterVaporTransmission rdf:type owl:DatatypeProperty ;
                              rdfs:domain ado:Substrate ;
                              rdfs:range xsd:float ;
                              rdfs:comment "A relation between a substrate and a minimum estimation of the passage of water vapor through it (in g*mm/m^2*day)" .


###  http://w3id.org/ado/organicSolventResistance
ado:organicSolventResistance rdf:type owl:DatatypeProperty ;
                             rdfs:subPropertyOf ado:environmentalResistance ;
                             rdfs:comment "A relation between an adhesive type or a substrate and its relative ability to withstand organic solvents" .


###  http://w3id.org/ado/peelResistance
ado:peelResistance rdf:type owl:DatatypeProperty ;
                   rdfs:domain ado:Adhesive ;
                   rdfs:range xsd:float ;
                   rdfs:comment "A relation between an adhesive and the peel resistance of its bonds (in N/mm)" .


###  http://w3id.org/ado/polymerType
ado:polymerType rdf:type owl:DatatypeProperty ;
                rdfs:domain ado:AdhesiveFamily ;
                rdfs:range xsd:string ;
                rdfs:comment "A relation between an adhesive type and its polymer type" .


###  http://w3id.org/ado/resinHardenerRatio
ado:resinHardenerRatio rdf:type owl:DatatypeProperty ;
                       rdfs:domain ado:Adhesive ;
                       rdfs:range xsd:float ;
                       rdfs:comment "A relation between an adhesive and its ratio between the volume of resin over the volume of hardener which should be mixed" .


###  http://w3id.org/ado/saltWaterResistance
ado:saltWaterResistance rdf:type owl:DatatypeProperty ;
                        rdfs:subPropertyOf ado:environmentalResistance ;
                        rdfs:comment "A relation between an adhesive type or substrate and its relative ability to withstand salt water" .


###  http://w3id.org/ado/sealingQuality
ado:sealingQuality rdf:type owl:DatatypeProperty ;
                   rdfs:domain ado:AdhesiveFamily ;
                   rdfs:range xsd:string ;
                   rdfs:comment "A relation between an adhesive family and its relative effectiveness in preventing the passage of air, moisture, dust or other substances through a bonded joint" .


###  http://w3id.org/ado/shearStrengthDegree
ado:shearStrengthDegree rdf:type owl:DatatypeProperty ;
                        rdfs:domain ado:AdhesiveFamily ;
                        rdfs:range xsd:string ;
                        rdfs:comment "A relation between an adhesive type and the degree of its shear strength, classified as low, medium or high" .


###  http://w3id.org/ado/shelfLife
ado:shelfLife rdf:type owl:DatatypeProperty ;
              rdfs:domain ado:Adhesive ;
              rdfs:range xsd:float ;
              rdfs:comment "A relation between an adhesive and its maximum recommended time it can be stored (in months)" .


###  http://w3id.org/ado/shockResistance
ado:shockResistance rdf:type owl:DatatypeProperty ;
                    rdfs:subPropertyOf ado:environmentalResistance ;
                    rdfs:comment "A relation between an adhesive type or substrate and its relative ability to withstand shock" .


###  http://w3id.org/ado/strongAlkalisResistance
ado:strongAlkalisResistance rdf:type owl:DatatypeProperty ;
                            rdfs:subPropertyOf ado:environmentalResistance ;
                            rdfs:comment "A relation between an adhesive type or substrate and its relative ability to withstand strong alkalis" .


###  http://w3id.org/ado/substrateMaxElongation
ado:substrateMaxElongation rdf:type owl:DatatypeProperty ;
                           rdfs:domain ado:Substrate ;
                           rdfs:range xsd:float ;
                           rdfs:comment "A relation between a substrate and the its maximum ductility. It is expressed as a percentage, and it is the maximum ratio of change in axial length with the application of a tensile force to the original length of the specimen" .


###  http://w3id.org/ado/substrateMaxYoungModulus
ado:substrateMaxYoungModulus rdf:type owl:DatatypeProperty ;
                             rdfs:domain ado:Substrate ;
                             rdfs:range xsd:float ;
                             rdfs:comment "A relation between a substrate and the maximum estimated tensile or compressive stiffness when the force is applied lengthwise (in GPa)" .


###  http://w3id.org/ado/substrateMinElongation
ado:substrateMinElongation rdf:type owl:DatatypeProperty ;
                           rdfs:domain ado:Substrate ;
                           rdfs:range xsd:float ;
                           rdfs:comment "A relation between a substrate and the its minimum ductility. It is expressed as a percentage, and it is the minimum ratio of change in axial length with the application of a tensile force to the original length of the specimen" .


###  http://w3id.org/ado/substrateMinYoungModulus
ado:substrateMinYoungModulus rdf:type owl:DatatypeProperty ;
                             rdfs:domain ado:Substrate ;
                             rdfs:range xsd:float ;
                             rdfs:comment "A relation between a substrate and the minimum estimated tensile or compressive stiffness when the force is applied lengthwise (in GPa)" .


###  http://w3id.org/ado/substrateTensileStrengthLowerBound
ado:substrateTensileStrengthLowerBound rdf:type owl:DatatypeProperty ;
                                       rdfs:domain ado:Substrate ;
                                       rdfs:range xsd:float ;
                                       rdfs:comment "A relation between a substrate and the lower bound of the maximum amount of stress it can withstand while being stretched or pulled before breaking (in MPa)" .


###  http://w3id.org/ado/substrateTensileStrengthUpperBound
ado:substrateTensileStrengthUpperBound rdf:type owl:DatatypeProperty ;
                                       rdfs:domain ado:Substrate ;
                                       rdfs:range xsd:float ;
                                       rdfs:comment "A relation between a substrate and the upper bound of the maximum amount of stress it can withstand while being stretched or pulled before breaking (in MPa)" .


###  http://w3id.org/ado/thermalConductivity
ado:thermalConductivity rdf:type owl:DatatypeProperty ;
                        rdfs:domain ado:Adhesive ,
                                    ado:Substrate ;
                        rdfs:range xsd:float ;
                        rdfs:comment "A relation between an adhesive or a substrate and an estimation of its ability to conduct heat (in W/m.°C)" .


###  http://w3id.org/ado/transparency
ado:transparency rdf:type owl:DatatypeProperty ;
                 rdfs:domain ado:Substrate ;
                 rdfs:range xsd:string ;
                 rdfs:comment "A relation between a substrate and a its quality of allowing light to pass through so that objects behind can be distinctly seen" .


###  http://w3id.org/ado/uvResistance
ado:uvResistance rdf:type owl:DatatypeProperty ;
                 rdfs:subPropertyOf ado:environmentalResistance ;
                 rdfs:comment "A relation between an adhesive type or a substrate and its relative ability to withstand uv radiation" .


###  http://w3id.org/ado/vibrationsDamping
ado:vibrationsDamping rdf:type owl:DatatypeProperty ;
                      rdfs:domain ado:AdhesiveFamily ;
                      rdfs:range xsd:string ;
                      rdfs:comment "A relation between an adhesive family and its relative ability to absorve vibrational energy" .


###  http://w3id.org/ado/viscosityTemperatureValidity
ado:viscosityTemperatureValidity rdf:type owl:DatatypeProperty ;
                                 rdfs:domain ado:Adhesive ;
                                 rdfs:range xsd:float ;
                                 rdfs:comment "A relation between an adhesive and the temperature validity of its viscosity in °C" .


###  http://w3id.org/ado/waterResistance
ado:waterResistance rdf:type owl:DatatypeProperty ;
                    rdfs:subPropertyOf ado:environmentalResistance ;
                    rdfs:comment "A relation between an adhesive type or substrate and its relative ability to resist water" .


###  http://w3id.org/ado/youngModulus
ado:youngModulus rdf:type owl:DatatypeProperty ;
                 rdfs:domain ado:Adhesive ;
                 rdfs:range xsd:float .


#################################################################
#    Classes
#################################################################

###  http://schema.org/Brand
schema:Brand rdf:type owl:Class .


###  http://schema.org/Product
schema:Product rdf:type owl:Class .


###  http://w3id.org/ado/AdhesionApplication
ado:AdhesionApplication rdf:type owl:Class ;
                        rdfs:comment "A task that an addhesive is typically used in." .


###  http://w3id.org/ado/AdhesionQuality
ado:AdhesionQuality rdf:type owl:Class ;
                    rdfs:comment "A quality estimation of an adhesive type" .


###  http://w3id.org/ado/Adhesive
ado:Adhesive rdf:type owl:Class ;
             rdfs:subClassOf schema:Product ;
             rdfs:comment "A non-metallic substance applied to one or both surface of two separate items that binds them together and resists their separation" .


###  http://w3id.org/ado/AdhesiveFamily
ado:AdhesiveFamily rdf:type owl:Class ;
                   rdfs:comment "A family of common adhesives, categorized by method of adhesion." .


###  http://w3id.org/ado/Industry
ado:Industry rdf:type owl:Class ;
             rdfs:comment "A generally categorized brand of economic activity" .


###  http://w3id.org/ado/MaterialFamily
ado:MaterialFamily rdf:type owl:Class ;
                   rdfs:comment "A category of materials that a substrate belongs in" .


###  http://w3id.org/ado/Solvent
ado:Solvent rdf:type owl:Class ;
            rdfs:comment "A substance that dissolves a solute, resulting in a solution" .


###  http://w3id.org/ado/Substrate
ado:Substrate rdf:type owl:Class ;
              rdfs:comment "A material surface" .


###  https://w3id.org/pmd/co/PMD_0000000
pmd:PMD_0000000 rdf:type owl:Class ;
                rdfs:label "Material" .


###  Generated by the OWL API (version 4.5.9.2019-02-01T07:24:44Z) https://github.com/owlcs/owlapi
